backends/lean/Aeneas/Std/Core/FmtWithSlice.lean
@@ -8,7 +8,7 @@ namespace Aeneas.Std
 def core.fmt.Formatter.debug_struct_fields_finish :
   core.fmt.Formatter → Str → Slice Str →
     Slice (Dyn (fun _dyn => core.fmt.Debug _dyn)) →
-    Result ((core.result.Result Unit core.fmt.Error) × core.fmt.Formatter) :=
+    RustM ((core.result.Result Unit core.fmt.Error) × core.fmt.Formatter) :=
   -- TODO: more precise model
   fun fmt _ _ _ =>
   .ok (.Ok (), fmt)
