backends/lean/Aeneas/Std/Std/Io.lean
@@ -3,6 +3,6 @@ import Aeneas.Std.Core.Fmt
 namespace Aeneas.Std
 
 @[rust_fun "std::io::stdio::_print"]
-def std.io.stdio._print (_ : core.fmt.Arguments) : Result Unit := .ok ()
+def std.io.stdio._print (_ : core.fmt.Arguments) : RustM Unit := .ok ()
 
 end Aeneas.Std
